\section{ Mathematics }

\subsection{ Important Sums }
\begingroup
\allowdisplaybreaks
\begin{flalign}
      & \sum_{i=0}^{n} \binom{n}{i} a^{n-i} b^i    = (a+b)^n                                               &  & \\
      & \sum_{i=0}^{n} \binom{n}{i}                = 2^n                                                   &  & \\
      & \sum_{i=0}^{n} \binom{i}{k}                = \binom{n+1}{k+1}                                      &  & \\
      & \sum_{i=0}^{n} i \binom{n}{i}              = n 2^{n-1}                                             &  & \\
      & \sum_{i=0}^{n} \frac{\binom{n}{i}}{i+1}    = \frac{2^{n+1} - 1}{n+1}                               &  & \\
      & \sum_{i=0}^{n} i! \binom{n}{i}             = \left\lfloor n! \cdot e \right\rfloor                 &  & \\
      & \sum_{i=0}^{n} {}_i P_k \binom{n}{i}       = {}_n P_k (2^{n-k})                                    &  & \\
      & \sum_{i=0}^{n} i \cdot i!                  = (n+1)! - 1                                            &  & \\
      & \sum_{k=0}^{m} \binom{n+k}{n}              = \binom{n+m+1}{n+1}                                    &  & \\
      & \sum_{i=0}^{n} \binom{n}{i}^2              = \binom{2n}{n}                                         &  & \\
      & \sum_{i=0}^{n} \frac{1}{i!}                = \frac{\left\lfloor n! \cdot e \right\rfloor}{n!}      &  & \\
      & \sum_{i=0}^{n} i P_k \binom{n}{i} = P_k (2^{n-k})                                                  &  & \\
      & \sum_{i=1}^{n} i + k P_{k+1} = \sum_{i=1}^{n} \prod_{j=0}^{k} (i+j) = \frac{(n+k+1)!}{(n-1)!(k+2)} &  & \\
      & \sum_{i=0}^{n} i! \cdot \binom{n}{i} = \sum_{i=0}^{n} P_{n}{i} = \lfloor n! \cdot e \rfloor        &  &
\end{flalign}
\endgroup

\newcolumn

\subsection{ Matrix }
\importcode{code/Matrix/matrix.h}

\newcolumn

\pausecol
\addcontentsline{toc}{subsection}{ Distribution table }
\begin{center}
     \renewcommand{\arraystretch}{2.2}
     \begin{tabular}{cccccc}
          \textbf{Distribution} & \textbf{PMF/PDF and Support} & \textbf{Expected Value} & \textbf{Variance} & \textbf{MGF} \\
          \hline
          \shortstack{Bernoulli                                                                                             \\ \Bern($p$)} & \shortstack{$P(X=1) = p$ \\$ P(X=0) = q=1-p$} & $p$ & $pq$ & $q + pe^t$ \\
          \hline
          \shortstack{Binomial                                                                                              \\ \Bin($n, p$)} & \shortstack{$P(X=k) = {n \choose k}p^k q^{n-k}$  \\ $k \in \{0, 1, 2, \dots n\}$}& $np$ & $npq$ & $(q + pe^t)^n$ \\
          \hline
          \shortstack{Geometric                                                                                             \\ \Geom($p$)} & \shortstack{$P(X=k) = q^kp$  \\ $k \in \{$0, 1, 2, \dots $\}$}& $q/p$ & $q/p^2$ & $\frac{p}{1-qe^t}, \, qe^t < 1$\\
          \hline
          \shortstack{Negative Binomial                                                                                     \\ \NBin($r, p$)} & \shortstack{$P(X=n) = {r + n - 1 \choose r -1}p^rq^n$ \\ $n \in \{$0, 1, 2, \dots $\}$} & $rq/p$ & $rq/p^2$ &  $(\frac{p}{1-qe^t})^r, \, qe^t < 1$\\
          \hline
          \shortstack{Hypergeometric                                                                                        \\ \Hypergeometric($w, b, n$)} & \shortstack{$P(X=k) = \sfrac{{w \choose k}{b \choose n-k}}{{w + b \choose n}}$ \\ $k \in \{0, 1, 2, \dots,  n\}$} & $\mu = \frac{nw}{b+w}$ &$\left(\frac{w+b-n}{w+b-1} \right) n\frac{\mu}{n}(1 - \frac{\mu}{n})$& messy  \\
          \hline
          \shortstack{Poisson                                                                                               \\ \Pois($\lambda$)} & \shortstack{$P(X=k) = \frac{e^{-\lambda}\lambda^k}{k!}$ \\ $k \in \{$0, 1, 2, \dots $\}$} & $\lambda$ & $\lambda$ & $e^{\lambda(e^t-1)}$ \\
          \hline
          \hline
          \shortstack{Uniform                                                                                               \\ \Unif($a, b$)} & \shortstack{$ f(x) = \frac{1}{b-a}$ \\$ x \in (a, b) $} & $\frac{a+b}{2}$ & $\frac{(b-a)^2}{12}$ &  $\frac{e^{tb}-e^{ta}}{t(b-a)}$\\
          \hline
          \shortstack{Normal                                                                                                \\ $\N(\mu, \sigma^2)$} & \shortstack{$f(x) = \frac{1}{\sigma \sqrt{2\pi}} e^{-\sfrac{(x - \mu)^2}{(2 \sigma^2)}}$ \\ $x \in (-\infty, \infty)$} & $\mu$  & $\sigma^2$ & $e^{t\mu + \frac{\sigma^2t^2}{2}}$\\
          \hline
          \shortstack{Exponential                                                                                           \\ $\Expo(\lambda)$} & \shortstack{$f(x) = \lambda e^{-\lambda x}$\\$ x \in (0, \infty)$} & $\frac{1}{\lambda}$  & $\frac{1}{\lambda^2}$ & $\frac{\lambda}{\lambda - t}, \, t < \lambda$\\
          \hline
          \shortstack{Gamma                                                                                                 \\ $\Gam(a, \lambda)$} & \shortstack{$f(x) = \frac{1}{\Gamma(a)}(\lambda x)^ae^{-\lambda x}\frac{1}{x}$\\$ x \in (0, \infty)$} & $\frac{a}{\lambda}$  & $\frac{a}{\lambda^2}$ & $\left(\frac{\lambda}{\lambda - t}\right)^a, \, t < \lambda$\\
          \hline
          \shortstack{Beta                                                                                                  \\ \Beta($a, b$)} & \shortstack{$f(x) = \frac{\Gamma(a+b)}{\Gamma(a)\Gamma(b)}x^{a-1}(1-x)^{b-1}$\\$x \in (0, 1) $} & $\mu = \frac{a}{a + b}$  & $\frac{\mu(1-\mu)}{(a + b + 1)}$ & messy \\
          \hline
          \shortstack{Log-Normal                                                                                            \\ $\mathcal{LN}(\mu,\sigma^2)$} & \shortstack{$\frac{1}{x\sigma \sqrt{2\pi}}e^{-(\log x - \mu)^2/(2\sigma^2)}$\\$x \in (0, \infty)$} & $\theta = e^{ \mu + \sigma^2/2}$ & $\theta^2 (e^{\sigma^2} - 1)$ & doesn't exist\\
          \hline
          \shortstack{Chi-Square                                                                                            \\ $\chi_n^2$} & \shortstack{$\frac{1}{2^{n/2}\Gamma(n/2)}x^{n/2 - 1}e^{-x/2}$\\$x \in (0, \infty) $} & $n$  & $2n$ & $(1 - 2t)^{-n/2}, \, t < 1/2$\\
          \hline
          \shortstack{Student-$t$                                                                                           \\ $t_n$} & \shortstack{$\frac{\Gamma((n+1)/2)}{\sqrt{n\pi} \Gamma(n/2)} (1+x^2/n)^{-(n+1)/2}$\\$x \in (-\infty, \infty)$} & $0$ if $n>1$ & $\frac{n}{n-2}$ if $n>2$ & doesn't exist\\
          \hline
     \end{tabular}
\end{center}
\clearpage
\resumecol
